theories/heap.v
@@ -23,15 +23,14 @@ Definition sem_typeOF (F: oFunctor) : oFunctor := value -d> F.
 
 (* The semantic heap is a map from locations to:
  * - a runtime tag
- * - the list of types used at the `alloc` site to instantiate the generics
  * - the (gated by Next) interpretation of fields for this tag
  *)
 Class sem_heapGpreS (Σ : gFunctors) : Set := {
-  sem_heap :> inG Σ (gmap_viewR loc (prodO tagO (prodO (listO lang_tyO) (gmapO string (laterO (sem_typeO Σ))))));
+  sem_heap :> inG Σ (gmap_viewR loc (prodO tagO (gmapO string (laterO (sem_typeO Σ)))));
 }.
 
 Definition sem_heapΣ : gFunctors :=
-  #[GFunctor (gmap_viewRF loc (tagO * ((listOF lang_tyO) * (gmapOF string (laterOF (sem_typeOF ∙))))))].
+  #[GFunctor (gmap_viewRF loc (tagO * (gmapOF string (laterOF (sem_typeOF ∙)))))].
 
 Global Instance subG_sem_heapΣ {Σ}: subG sem_heapΣ Σ → sem_heapGpreS Σ.
 Proof.  solve_inG. Qed.
@@ -45,14 +44,12 @@ Section definitions.
   Context `{hG: !sem_heapGS Σ}.
 
   Definition loc_mapsto_def (ℓ: loc) (t: tag)
-    (σ : listO lang_tyO)
     (iFs: gmapO string (laterO (sem_typeO Σ))) :=
-    (gmap_view_frag ℓ DfracDiscarded (t, (σ, iFs))).
+    (gmap_view_frag ℓ DfracDiscarded (t, iFs)).
 
   Definition mapsto_def (ℓ: loc) (t: tag)
-    (σ : listO lang_tyO)
     (iFs: gmapO string (laterO (sem_typeO Σ))) :=
-    own (@sem_heap_name _ hG) (loc_mapsto_def ℓ t σ iFs).
+    own (@sem_heap_name _ hG) (loc_mapsto_def ℓ t iFs).
 
   Definition loc_mapsto_aux : seal (@loc_mapsto_def). Proof. by eexists. Qed.
   Definition loc_mapsto := loc_mapsto_aux.(unseal).
@@ -63,25 +60,25 @@ Section definitions.
   Definition mapsto_eq : @mapsto = @mapsto_def := mapsto_aux.(seal_eq).
 End definitions.
 
-Notation "l ↪ '(' t ',' σ ',' iFs ')'" := (loc_mapsto l t σ iFs)
-  (at level 20, format "l  ↪ '(' t ',' σ ',' iFs ')'") : bi_scope.
+Notation "l ↪ '(' t ',' iFs ')'" := (loc_mapsto l t iFs)
+  (at level 20, format "l  ↪ '(' t ',' iFs ')'") : bi_scope.
 
-Notation "l ↦ '(' t ',' σ ',' iFs ')'" := (mapsto l t σ iFs)
-  (at level 20, format "l ↦ '(' t ',' σ ',' iFs ')'") : bi_scope.
+Notation "l ↦ '(' t ',' iFs ')'" := (mapsto l t iFs)
+  (at level 20, format "l ↦ '(' t ',' iFs ')'") : bi_scope.
 
 Section sem_heap.
   Context `{hG: !sem_heapGS Σ}.
   Notation γ := sem_heap_name.
 
-  Global Instance mapsto_persistent l t σ iFs: Persistent (mapsto l t σ iFs).
+  Global Instance mapsto_persistent l t iFs: Persistent (mapsto l t iFs).
   Proof.
     rewrite mapsto_eq /mapsto_def /loc_mapsto_def.
     by apply _.
   Qed.
 
-  Lemma mapsto_proper l t σ iFs0 iFs1 :
+  Lemma mapsto_proper l t iFs0 iFs1 :
     iFs0 ≡ iFs1 →
-    mapsto l t σ iFs0 ≡ mapsto l t σ iFs1.
+    mapsto l t iFs0 ≡ mapsto l t iFs1.
   Proof.
     move => heq.
     rewrite mapsto_eq /mapsto_def /loc_mapsto_def.
@@ -89,10 +86,10 @@ Section sem_heap.
     by f_equiv.
   Qed.
 
-  Lemma sem_heap_own_valid_2 sh l t σ iFs:
+  Lemma sem_heap_own_valid_2 sh l t iFs:
     own γ (gmap_view_auth (DfracOwn 1) sh) -∗
-    l ↦ (t, σ, iFs) -∗
-    sh !! l ≡ Some (t, (σ, iFs)).
+    l ↦ (t, iFs) -∗
+    sh !! l ≡ Some (t, iFs).
   Proof.
     rewrite mapsto_eq /mapsto_def /loc_mapsto_def.
     iIntros "H● H◯".
@@ -101,28 +98,28 @@ Section sem_heap.
     by iDestruct "Hv" as "[_ HΦ]".
   Qed.
 
-  Lemma sem_heap_view_alloc sh new t σ iFs:
+  Lemma sem_heap_view_alloc sh new t iFs:
     sh !! new = None →
     gmap_view_auth (DfracOwn 1) sh ~~>
-    gmap_view_auth (DfracOwn 1) (<[new:=(t, (σ, iFs))]> sh) ⋅ (@loc_mapsto Σ new t σ iFs).
+    gmap_view_auth (DfracOwn 1) (<[new:=(t, iFs)]> sh) ⋅ (@loc_mapsto Σ new t iFs).
   Proof.
     move => hnew.
     rewrite loc_mapsto_eq /loc_mapsto_def.
     by apply gmap_view_alloc.
   Qed.
 
-  Lemma sem_heap_own_update new sh t σ iFs:
+  Lemma sem_heap_own_update new sh t iFs:
     sh !! new = None →
     (gmap_view_auth (DfracOwn 1) sh ~~>
-      gmap_view_auth (DfracOwn 1) (<[new:=(t, (σ, iFs))]> sh) ⋅ (new ↪ (t, σ, iFs))%I) →
+      gmap_view_auth (DfracOwn 1) (<[new:=(t, iFs)]> sh) ⋅ (new ↪ (t, iFs))%I) →
     own γ (gmap_view_auth (DfracOwn 1) sh) -∗
-    |==> (own γ (gmap_view_auth (DfracOwn 1) (<[new:=(t, (σ, iFs))]> sh))) ∗
-         (new ↦ (t, σ, iFs))%I.
+    |==> (own γ (gmap_view_auth (DfracOwn 1) (<[new:=(t, iFs)]> sh))) ∗
+         (new ↦ (t, iFs))%I.
   Proof.
     rewrite loc_mapsto_eq /loc_mapsto_def  => hnew h.
     iIntros "H●".
     iMod (own_update with "H●") as "[? ?]";
-      first by apply (gmap_view_alloc _ new DfracDiscarded (t, (σ, iFs))).
+      first by apply (gmap_view_alloc _ new DfracDiscarded (t, iFs)).
     iModIntro.
     iSplit; first done.
     by rewrite mapsto_eq /mapsto_def /loc_mapsto_def.
